Procedure calls are defined inductively and functionaly, and bisimulate.
Currently a naive stack policy is applied, which does not keep the
stack at the same size as the typing stack.

completeness results and typing results are not yet proved for
procedures, and therefore do not compile at all.

language_formal/spark2014_semantics/language.v
@@ -191,6 +191,10 @@ Definition procedure_parameter_profile pb :=
 match pb with
   | mkprocedure_body _ _ _ x _ _ => x
 end.
+Definition procedure_name pb :=
+match pb with
+  | mkprocedure_body _ x _ _ _ _ => x
+end.
 
 
 (* Declarations are of two kinds and can be sequenced *)
@@ -219,3 +223,28 @@ Inductive library_unit_declaration: Type :=
 (* 10.1.1 *)
 Inductive compilation_unit: Type := 
 	| Library_Unit: astnum -> library_unit_declaration -> type_table -> compilation_unit.
+
+(** Some useful definition, related to language structures *)
+
+(** [Is_var e] means that expression [e] is a variable *)
+Definition Is_var e:Prop :=
+  match e with
+    |  E_Identifier _ _ => True
+    | _ => False
+  end.
+
+(** functional version of Is_var above *)
+Definition is_var e:bool :=
+  match e with
+    |  E_Identifier _ _ => true
+    | _ => false
+  end.
+
+(** correctness of is_var. *)
+Lemma is_var_Is_var : forall e, is_var e = true <-> Is_var e.
+Proof.
+  intros e.
+  destruct e;simpl; split;intro h;auto;try contradiction; discriminate h. 
+Qed.
+
+
