language_formal/spark2014_semantics/util.v
@@ -91,9 +91,158 @@ Ltac distr_qualifier :=
             ; [split; intros xz; specialize (h xz); rm_exists; assumption | ]; clear h; rm_exists
     end.
 
+Require Import List.
+(* Functional Scheme lgth_ind := Induction for Datatypes.length Sort Prop. *)
 
 
+Lemma length_invnil : forall A (l:list A), length l = 0 -> l = nil.
+Proof.
+  intros A l H.
+  destruct l;auto;simpl in *.
+  inversion H.
+Qed.
 
+Lemma length_invcons : forall A n (l:list A), length l = S n -> exists x l', l = x::l'.
+Proof.
+  intros A n l H.
+  destruct l;auto;simpl in *.
+  inversion H.
+  exists a.
+  exists l.
+  reflexivity.
+Qed.
+
+Function split1 A n (l:list A) {struct n} :=
+  match l,n with
+    | _,O => Some(nil,l)
+    | e::l' , S n'  =>
+      match split1 A n' l' with
+        | Some(l1,l2) => Some (e::l1,l2)
+        | None => None
+      end
+    | nil, S _ => None
+  end.
+
+(* This should be a regular Definition but it makes Function bug
+   later, this is a bug of Function that will be hopefukly fixed in
+   next versions. *)
+Definition split2 {A} n m (l:list A) :=
+  match split1 A n l with
+    | None => None
+    | Some (l1,l2') =>
+      match split1 A m l2' with
+        | None => None
+        | Some (l2,l3) => Some (l1,(l2,l3))
+      end
+  end.
+
+
+Lemma split1_correct :
+  forall A n (l l2 l1:list A),
+    (split1 _ n l = Some (l1,l2))
+    -> List.length l1 = n /\ (l = l1 ++ l2).
+Proof.
+  intros A n l.
+  functional induction split1 A n l;simpl;intros.
+  - inversion H.
+    clear H.
+    subst.
+    simpl.
+    split; reflexivity.
+  - inversion H.
+    clear H.
+    subst.
+    specialize (IHo _ _ e2).
+    destruct IHo as [IHo1 IHo2].
+    subst.
+    split;reflexivity.
+  - inversion H.
+  - inversion H.
+Qed.
+
+
+Lemma split1_correct_eq :
+  forall A n (l l2 l1:list A),
+    (split1 _ n l = Some (l1,l2))
+    -> (l = l1 ++ l2).
+Proof.
+  intros A n l l2 l1 H.
+  apply (split1_correct A n l l2 l1) in H.
+  destruct H;assumption.
+Qed.
+
+Lemma split1_correct_length :
+  forall A n (l l2 l1:list A),
+    (split1 _ n l = Some (l1,l2))
+    -> List.length l1 = n.
+Proof.
+  intros A n l l2 l1 H.
+  apply (split1_correct A n l l2 l1) in H.
+  destruct H;assumption.
+Qed.
+
+
+Lemma split1_complete :
+  forall A n (l l2 l1:list A),
+    List.length l1 = n
+    -> (l = l1 ++ l2)
+    -> (split1 _ n l = Some (l1,l2)).
+Proof.
+  intros A n l.
+  functional induction split1 A n l;simpl;intros.
+  - rewrite (length_invnil _ _ H) in *.
+    simpl in *.
+    subst.
+    reflexivity.
+  - destruct (length_invcons _ _ _ H) as [e' l''].
+    destruct l''.
+    subst.
+    simpl in *.
+    inversion H; clear H.
+    inversion H0. clear H0.
+    subst.
+    specialize (IHo l0 x refl_equal refl_equal).
+    rewrite e2 in IHo.
+    inversion IHo.
+    reflexivity.
+  - destruct l1.
+    + simpl in *.
+      discriminate.
+    + simpl in *.
+      inversion  H0.
+      specialize (IHo l2 l1).
+      rewrite IHo in e2;try discriminate.
+      * inversion H.
+        reflexivity.
+      * assumption.
+  - apply length_invcons in H.
+    decompose [ex] H. clear H.
+    subst.
+    simpl in *.
+    inversion H0.
+Qed.
+
+Lemma split2_correct :
+  forall A n m (l l1 l2 l3:list A),
+    split2 n m l = Some (l1,(l2,l3))
+    -> (l = l1 ++ l2 ++ l3) /\ List.length l1 = n /\ List.length l2 = m.
+Proof.
+  intros A n m l l1 l2 l3 H.
+  unfold split2 in H.
+  destruct (split1 A n l) eqn:heq.
+  - destruct p.
+    apply split1_correct in heq.
+    destruct heq as [heq1 heq2].
+    subst l.
+    destruct (split1 A m l4) eqn:heq'.
+    + destruct p.
+      inversion H;clear H;subst. 
+      apply split1_correct in heq'.
+      destruct heq' as [heq'1 heq'2].
+      subst;auto.
+    + inversion H.
+  - inversion H.
+Qed.
 
 
 
